CollapsingTowers/Stlc/Basic.lean
@@ -1,0 +1,11 @@
+
+inductive Expr : Type where
+  | bvar (i : Nat)
+  | fvar (x : String)
+  | lam (e : Expr)
+  | app (f : Expr) (arg : Expr)
+  | unit
+
+inductive value : Expr -> Prop where
+  | value_lam : value (.lam e)
+  | value_unit : value .unit
