CollapsingTowers/Stlc/OpenClose.lean
@@ -1,0 +1,27 @@
+
+import CollapsingTowers.Stlc.Basic
+@[simp]
+def subst (x : String) (v : Expr) : Expr -> Expr
+  | .bvar i => .bvar i
+  | .fvar y => if x == y then v else .fvar y
+  | .lam e => .lam (subst x v e)
+  | .app f arg => .app (subst x v f) (subst x v arg)
+  | .unit => .unit
+
+@[simp]
+def openRec (n : Nat) (v : Expr) : Expr -> Expr
+  | .bvar i => if n == i then v else .bvar i
+  | .fvar x => .fvar x
+  | .lam e => .lam (openRec (n + 1) v e)
+  | .app f arg => .app (openRec n v f) (openRec n v arg)
+  | .unit => .unit
+
+@[simp]
+def open₀ (v : Expr) : Expr -> Expr :=
+  openRec 0 v
+
+inductive lc : Expr -> Prop where
+  | lc_fvar : lc (.fvar x)
+  | lc_lam : lc (open₀ e x) -> lc (.lam e)
+  | lc_app : lc f -> lc arg -> lc (.app f arg)
+  | lc_unit : lc .unit
