CollapsingTowers/Stlc/Typing.lean
@@ -1,0 +1,113 @@
+
+import Mathlib.Data.Finset.Basic
+import CollapsingTowers.Stlc.Basic
+import CollapsingTowers.Stlc.OpenClose
+import CollapsingTowers.Stlc.SmallStep
+inductive Ty : Type where
+  | ty_unit
+  | ty_fun : Ty -> Ty -> Ty
+
+abbrev TyCtx :=
+  List (String × Ty)
+
+@[simp]
+def lookup (Γ : TyCtx) (x : String) : Option Ty :=
+  match Γ with
+  | [] => none
+  | (y, τ) :: Γ => if x = y then some τ else lookup Γ x
+
+@[simp]
+def in_context (x : String) : TyCtx → Prop
+  | [] => False
+  | ((y, _) :: Γ) => (x = y) ∨ (in_context x Γ)
+
+@[simp]
+def context_terms : TyCtx → (Finset String)
+  | [] => ∅
+  | ((x, _) :: Γ) => { x } ∪ (context_terms Γ)
+
+inductive ok : TyCtx → Prop where
+  | ok_nil : ok []
+  | ok_cons : ok Γ → ¬(in_context x Γ) → ok ((x, τ) :: Γ)
+
+inductive hasTy : TyCtx -> Expr -> Ty -> Prop
+  | hasTy_var : ok Γ -> lookup Γ x = some τ -> hasTy Γ (.fvar x) τ
+  |
+  hasTy_lam :
+    (L : Finset String) ->
+      (∀ x, x ∉ L -> hasTy ((x, τ₀) :: Γ) (open₀ (.fvar x) e) τ₁) -> hasTy Γ (.lam e) (.ty_fun τ₀ τ₁)
+  | hasTy_app : hasTy Γ f (.ty_fun τ₀ τ₁) -> hasTy Γ arg τ₀ -> hasTy Γ (.app f arg) τ₁
+  | hasTy_unit : hasTy Γ .unit .ty_unit
+
+theorem context_terms_iff_in_list : x ∈ context_terms Γ ↔ in_context x Γ :=
+  by
+  induction Γ
+  case nil => simp
+  case cons _ _ IH =>
+    simp
+    rw [IH]
+
+theorem hasTy_mono : hasTy Γ₀ e τ -> ok (Γ₀ ++ Γ₁) -> hasTy (Γ₀ ++ Γ₁) e τ :=
+  by
+  intro HhasTy HokΓ
+  induction HhasTy with
+  | @hasTy_var Γ₀ x _ HokΓ₀ Hlookup =>
+    constructor
+    apply HokΓ
+    induction Γ₀ with
+    | nil => simp at *
+    | cons head tails IHtails =>
+      simp at *
+      if HEq : x = head.fst then
+        rw [HEq] at Hlookup
+        rw [HEq]
+        simp at *
+        apply Hlookup
+      else
+        cases HokΓ₀ with
+        | ok_cons HokTailsΓ₀ =>
+          cases HokΓ with
+          | ok_cons HokTailsΓ =>
+            rw [if_neg HEq] at Hlookup
+            rw [if_neg HEq]
+            apply IHtails
+            apply HokTailsΓ₀
+            apply Hlookup
+            apply HokTailsΓ
+  | @hasTy_lam _ Γ₀ _ _ L _
+    IHhasTyE =>
+    apply hasTy.hasTy_lam (L ∪ context_terms (Γ₀ ++ Γ₁))
+    intro x HnotInL
+    simp at HnotInL
+    apply IHhasTyE
+    apply HnotInL.left
+    constructor
+    apply HokΓ
+    intro HinΓ
+    apply HnotInL.right
+    apply (context_terms_iff_in_list.mpr)
+    apply HinΓ
+  | hasTy_app _ _ IHhasTyF IHhasTyArg =>
+    constructor
+    apply IHhasTyF
+    apply HokΓ
+    apply IHhasTyArg
+    apply HokΓ
+  | hasTy_unit => constructor
+
+theorem preservation : step e₀ e₁ -> hasTy [] e₀ τ -> hasTy [] e₁ τ :=
+  by
+  intro Hstep
+  cases Hstep with
+  | step_appβ HM HV =>
+    induction HM with
+    | ctx𝕄_hole =>
+      simp
+      intro HhasTy
+      cases HhasTy with
+      | hasTy_app HhasTyF HhasTyArg =>
+        cases HhasTyF with
+        | hasTy_lam =>
+          simp at *
+          admit
+    | ctx𝕄_𝔹 => admit
