Makefile
@@ -1,11 +1,11 @@
-SRCS = $(wildcard CollapsingTowers/*.lean)
+SRCS = $(shell find CollapsingTowers -type f -name "*.lean")
 fmt:
 	@for file in $(SRCS); do \
 		echo "Processing $$file:"; \
-		sed -i '1,/^[^ \t]*import / s/^\(import\)/-- \1/' $$file; \
+		sed -i 's/^import/-- import/' $$file; \
 		sed -i 's/\blemma\b/theorem/g' $$file; \
 		lean --run script/Reformat.lean $$file | sponge $$file; \
-		sed -i 's/^--[ \t]*import/import/' $$file; \
+		sed -i 's/^-- import/import/' $$file; \
 		sed -i 's/[[:space:]]\+$$//' $$file; \
 		sed -i -e :a -e '/^\n*$$/{$$d;N;};/\n$$/ba' $$file; \
 	done
